Chess/Display.lean
@@ -2,18 +2,18 @@ import Chess.Model
 
 def Piece.toIcon (piece: Piece) (colour: Colour) : String :=
   match piece, colour with
-  | .king,   .white => "♔"
-  | .queen,  .white => "♕"
-  | .rook,   .white => "♖"
-  | .bishop, .white => "♗"
-  | .knight, .white => "♘"
-  | .pawn,   .white => "♙"
-  | .king,   .black => "♚"
-  | .queen,  .black => "♛"
-  | .rook,   .black => "♜"
-  | .bishop, .black => "♝"
-  | .knight, .black => "♞"
-  | .pawn,   .black => "♟"
+  | .king,   .white => "♚"
+  | .queen,  .white => "♛"
+  | .rook,   .white => "♜"
+  | .bishop, .white => "♝"
+  | .knight, .white => "♞"
+  | .pawn,   .white => "♟"
+  | .king,   .black => "♔"
+  | .queen,  .black => "♕"
+  | .rook,   .black => "♖"
+  | .bishop, .black => "♗"
+  | .knight, .black => "♘"
+  | .pawn,   .black => "♙"
 
 def Square.toIcon (square: Square) : String :=
   match square with
